

# Digital Logic Systems

## Recitation 5: Propositional Logic & Asymptotics

Guy Even    Moti Medina

School of Electrical Engineering Tel-Aviv Univ.

November 29, 2011

---

**Algorithm 1**  $\text{DM}(\varphi)$  - An algorithm for evaluating the De Morgan dual of a Boolean formula  $\varphi \in \mathcal{BF}(\{X_1, \dots, X_n\}, \{\neg, \text{OR}, \text{AND}\})$ .

---

- ① **Base Cases:** (parse tree of size 1 or 2)
    - ① If  $\varphi = 0$ , then return 1.
    - ② If  $\varphi = 1$ , then return 0.
    - ③ If  $\varphi = X_i$ , then return  $(\neg X_i)$ .
    - ④ If  $\varphi = (\neg 0)$ , then return 0.
    - ⑤ If  $\varphi = (\neg 1)$ , then return 1.
    - ⑥ If  $\varphi = (\neg X_i)$ , then return  $X_i$ .
  - ② **Reduction Rules:** (parse tree of size at least 3)
    - ① If  $\varphi = (\neg \varphi_1)$ , then return  $(\neg \text{DM}(\varphi_1))$ .
    - ② If  $\varphi = (\varphi_1 \cdot \varphi_2)$ , then return  $(\text{DM}(\varphi_1) + \text{DM}(\varphi_2))$ .
    - ③ If  $\varphi = (\varphi_1 + \varphi_2)$ , then return  $(\text{DM}(\varphi_1) \cdot \text{DM}(\varphi_2))$ .
- 

## Example

$\text{DM}(\neg(X + Y)) = ?$

## The De Morgan dual (cont.)

### Theorem

*For every Boolean formula  $\varphi$ ,  $DM(\varphi)$  is logically equivalent to  $(\neg\varphi)$ .*

# Revisiting De Morgan's Law for Sets

Recall that the De-Morgan's law states that for sets  $A, B$ ,

$$U \setminus (A \cup B) = \bar{A} \cap \bar{B}.$$

We depicted this law using Venn diagrams. We now prove this law, formally, using propositional logic.

Proof.

On the whiteboard.



# Negation Normal Form

A formula is in negation normal form if negation is applied only directly to **variables**.

## Definition

A Boolean formula  $\varphi \in \mathcal{BF}(\{X_1, \dots, X_n\}, \{\neg, \text{OR}, \text{AND}\})$  is in *negation normal form* if the parse tree  $(G, \pi)$  of  $\varphi$  satisfies the following condition. If a vertex in  $G$  is labeled by negation (i.e.,  $\pi(v) = \neg$ ), then  $v$  is a parent of a leaf labeled by a **variable**.

## Example

- The formula  $(\neg X) \cdot (\neg Y)$  is in negation normal form.
- The formulas  $(\neg 0)$ ,  $\neg(A \cdot B)$ ,  $\text{NOT}(\text{NOT}(X))$  are not in negation normal form.

## Theorem

*Let  $\varphi \in \mathcal{BF}(\{X_1, \dots, X_n\}, \{\neg, \text{OR}, \text{AND}\})$ . Then,  $\text{NNF}(\varphi)$  is logically equivalent to  $\varphi$  and in negation normal form.*

# Negation Normal Form (cont.)

---

**Algorithm 2**  $\text{NNF}(\varphi)$  - An algorithm for computing the negation normal form of a Boolean formula  $\varphi \in \mathcal{BF}(\{X_1, \dots, X_n\}, \{\neg, \text{OR}, \text{AND}\})$ .

---

- ① **Base Cases:** (parse tree of size 1 or 2)
    - ① If  $\varphi \in \{0, 1, X_i, (\neg X_i)\}$ , then return  $\varphi$ .
    - ② If  $\varphi = (\neg 0)$ , then return 1.
    - ③ If  $\varphi = (\neg 1)$ , then return 0.
  - ② **Reduction Rules:** (parse tree of size at least 3)
    - ① If  $\varphi = (\neg \varphi_1)$ , then return  $\text{DM}(\text{NNF}(\varphi_1))$ .
    - ② If  $\varphi = (\varphi_1 \cdot \varphi_2)$ , then return  $(\text{NNF}(\varphi_1) \cdot \text{NNF}(\varphi_2))$ .
    - ③ If  $\varphi = (\varphi_1 + \varphi_2)$ , then return  $(\text{NNF}(\varphi_1) + \text{NNF}(\varphi_2))$ .
- 

## Example

- $\text{NNF}(\neg\neg X) = ?$
- $\text{NNF}(\neg\neg\neg X) = ?$ .

## Definition (7)

Let  $f, g : \mathbb{N} \rightarrow \mathbb{R}^{\geq}$  denote two functions.

- 1 We say that  $g(n) = O(f(n))$ , if there exist constants  $c_1, c_2 \in \mathbb{R}^{\geq}$  such that, for every  $n \in \mathbb{N}$ ,

$$g(n) \leq c_1 \cdot f(n) + c_2.$$

- 2 We say that  $g(n) = \Omega(f(n))$ , if there exist constants  $c_3 \in \mathbb{R}^{>}$ ,  $c_4 \in \mathbb{R}^{\geq}$  such that, for every  $n \in \mathbb{N}$ ,

$$g(n) \geq c_3 \cdot f(n) + c_4.$$

- 3 We say that  $g(n) = \Theta(f(n))$ , if  $g(n) = O(f(n))$  and  $g(n) = \Omega(f(n))$ .

# Order of Growth: Alternative Definition

Let us consider the following alternative definition of order of growth.

## Definition (8)

Let  $f, g : \mathbb{N} \rightarrow \mathbb{R}^{\geq}$  denote two functions.

- 1 We say that  $g(n) = O(f(n))$ , if there exist constants  $c \in \mathbb{R}^{\geq}$  and  $N \in \mathbb{N}$ , such that, for every  $n \in \mathbb{N}$ ,

$$\forall n > N : g(n) \leq c \cdot f(n).$$

- 2 We say that  $g(n) = \Omega(f(n))$ , if there exist constants  $d \in \mathbb{R}^{>}$  and  $N \in \mathbb{N}$ , such that, for every  $n \in \mathbb{N}$ ,

$$\forall n > N : g(n) \geq d \cdot f(n).$$

- 3 We say that  $g(n) = \Theta(f(n))$ , if  $g(n) = O(f(n))$  and  $g(n) = \Omega(f(n))$ .



### Lemma

*Definitions 7 and 8 are equivalent if  $f(n) \geq 1$  and  $g(n) \geq 1$ , for every  $n$ .*

## Reminder: Is it enough to solve for powers of 2?

In the following lemma we show that, under reasonable conditions, it suffices to consider powers of two when bounding the rate of growth.

### Lemma (10)

*Assume that:*

- 1 The functions  $f(n)$  and  $g(n)$  are both monotonically nondecreasing.
- 2 The constant  $\rho$  satisfies, for every  $k \in \mathbb{N}$ ,

$$\rho \geq \frac{g(2^{k+1})}{g(2^k)}.$$

*If  $f(2^k) = O(g(2^k))$ , then  $f(n) = O(g(n))$ .*

## Revisiting: Is it enough to solve for powers of 2? Yes!

An analogous lemma that states that  $f(n) = \Omega(g(n))$  can be proved if  $\frac{g(2^{k+1})}{g(2^k)} \geq \rho$ , for a constant  $\rho$ . The lemma is as follows.

### Lemma

*Assume that:*

- 1 *The functions  $f(n)$  and  $g(n)$  are both monotonically nondecreasing.*
- 2 *The constant  $\rho$  satisfies, for every  $k \in \mathbb{N}$ ,*

$$\rho \leq \frac{g(2^{k+1})}{g(2^k)}.$$

*If  $f(2^k) = \Omega(g(2^k))$ , then  $f(n) = \Omega(g(n))$ .*

## Example - 1

Let  $g(n) \triangleq \log_3 n$ . We claim that  $g(n) = \Theta(\log_2 n)$

Proof.

Recall that for every  $a, b, c \in \mathbb{R}$ ,  $a, c \neq 1$ ,

$$\log_a b = \frac{\log_c b}{\log_c a}. \quad (1)$$

Hence,  $\log_3 n = \frac{\log_2 n}{\log_2 3}$ . Since,  $3/2 < \log_2 3 < 8/5$  is a constant, then  $c_1 = 2/3, c_2 = 0, c_3 = 5/8, c_4 = 0$  satisfy the conditions in Definition 7. □

Hence, when considering the order of growth of log functions with a constant base, that is  $\log_c n$  and  $\log_d n$  where  $c, d$  are constants, we may omit the base and simply refer the order of growth of these functions as  $O(\log n)$ ,  $\Omega(\log n)$  and  $\Theta(\log n)$ .

## Example - 2

Let  $g(n) \triangleq n^{\log_2 c}$ . We claim that  $g(n) = \Theta(c^{\log_2 n})$ .

Proof.

We prove the following stronger claim.

$$n^{\log_2 c} = c^{\log_2 n}. \quad (2)$$

That will conclude the proof, since for every two functions  $f, g : \mathbb{N} \rightarrow \mathbb{R}^{\geq}$ , if  $f = g$  then  $f(n) = \Theta(g(n))$  and  $g(n) = \Theta(f(n))$  (look for it in the text book!).

Let us apply the  $\log_2$  function on the left-hand side and the right-hand side of Eq. 2. We get

$$\begin{aligned} \log_2(n^{\log_2 c}) &\stackrel{?}{=} \log_2(c^{\log_2 n}) \Leftrightarrow \\ \log_2 c \cdot \log_2 n &= \log_2 n \cdot \log_2 c, \end{aligned} \quad (3)$$

where the second line follows from the fact that  $\log(a^b) = b \cdot \log(a)$ . Since Eq. 3 holds with equality, and since the  $\log$  function is one-to-one, then their arguments are equal as well,

## Example - 3: Recurrence 3.

Consider the recurrence

$$f(n) \triangleq \begin{cases} 1 & \text{if } n = 1 \\ n + 3 \cdot f(\lfloor \frac{n}{2} \rfloor) & \text{if } n > 1. \end{cases} \quad (4)$$

### Lemma

*The rate of growth of the function  $f(n)$  defined in Eq. 4 is  $\Theta(n^{\log_2 3})$ .*

### Proof.

On the whiteboard. □

## Example - 4

Consider the recurrence

$$f(n) \triangleq \begin{cases} c & \text{if } n = 1 \\ a \cdot n + b + f(\lfloor \frac{n}{2} \rfloor) & \text{if } n > 1, \end{cases} \quad (5)$$

where  $a, b, c$  are constants.

### Lemma

*The rate of growth of the function  $f(n)$  is  $\Theta(n)$ .*

proof:  $f(2^k) = 2a \cdot 2^k + b \cdot k + c - 2a \dots$

## Example -5

Consider the recurrence

$$f(n) \triangleq \begin{cases} c & \text{if } n = 1 \\ a \cdot n + b + 2 \cdot f(\lfloor \frac{n}{2} \rfloor) & \text{if } n > 1, \end{cases} \quad (6)$$

where  $a, b, c = O(1)$ .

### Lemma

*The rate of growth of the function  $f(n)$  is  $\Theta(n \log n)$ .*

proof: We claim that  $f(2^k) = a \cdot k 2^k + (b + c) \cdot 2^k - b \dots$



# Examples with floor and ceiling

1

$$f(n) \triangleq \begin{cases} 1 & \text{if } n = 1 \\ 1 + f(\lfloor \frac{n}{2} \rfloor) & \text{if } n > 1, \end{cases}$$

2

$$f(n) \triangleq \begin{cases} 1 & \text{if } n = 1 \\ n + f(\lfloor \frac{n}{2} \rfloor) + f(\lceil \frac{n}{2} \rceil) & \text{if } n > 1, \end{cases}$$